Figured out rules for RG algebra w/ operator

WeakTrioid/RelyGuarantee.thy
@@ -3,146 +3,123 @@ theory RelyGuarantee
 begin
 
 class rg_algebra = weak_trioid + meet_semilattice +
-  fixes I :: "'a set"
-  assumes inv1: "r \<in> I \<Longrightarrow> r \<parallel> r \<le> r"
-  and inv2: "r \<in> I \<Longrightarrow> s \<in> I \<Longrightarrow> r \<le> r \<parallel> s"
-  and inv3: "r \<in> I \<Longrightarrow> r\<parallel>(x\<cdot>y) = (r\<parallel>x)\<cdot>(r\<parallel>y)"
-  and inv4: "r \<in> I \<Longrightarrow> r\<parallel>x\<^sup>+ \<le> (r\<parallel>x)\<^sup>+"
-  and inv_unit: "1 \<in> I"
-  and inv_meet_closed: "\<lbrakk>r \<in> I; s \<in> I\<rbrakk> \<Longrightarrow> (r \<sqinter> s) \<in> I"
-  and inv_par_closed: "\<lbrakk>r \<in> I; s \<in> I\<rbrakk> \<Longrightarrow> (r \<parallel> s) \<in> I"
+  fixes RG :: "'a set"
+  and hom :: "'a \<Rightarrow> 'a" ("\<lbrakk>_\<rbrakk>")
+  assumes rg1: "r \<in> RG \<Longrightarrow> r \<parallel> r \<le> r"
+  and rg2: "r \<in> RG \<Longrightarrow> s \<in> RG \<Longrightarrow> r \<le> r \<parallel> s"
+  and rg3: "r \<in> RG \<Longrightarrow> r\<parallel>(x\<cdot>y) = (r\<parallel>x)\<cdot>(r\<parallel>y)"
+  and rg4: "r \<in> RG \<Longrightarrow> r\<parallel>x\<^sup>+ \<le> (r\<parallel>x)\<^sup>+"
+  and rg_unit: "1 \<in> RG"
+  and rg_meet_closed: "\<lbrakk>r \<in> RG; s \<in> RG\<rbrakk> \<Longrightarrow> (r \<sqinter> s) \<in> RG"
+  and rg_par_closed: "\<lbrakk>r \<in> RG; s \<in> RG\<rbrakk> \<Longrightarrow> (r \<parallel> s) \<in> RG"
+
+  and hom_iso: "x \<le> y \<Longrightarrow> \<lbrakk>x\<rbrakk> \<le> \<lbrakk>y\<rbrakk>"
+  and hom_meet: "\<lbrakk>x \<sqinter> y\<rbrakk> = \<lbrakk>x\<rbrakk> \<sqinter> \<lbrakk>y\<rbrakk>"
+  and hom_join [simp]: "\<lbrakk>x + y\<rbrakk> = \<lbrakk>x\<rbrakk> + \<lbrakk>y\<rbrakk>"
+  and hom_mult: "\<lbrakk>x\<cdot>y\<rbrakk> = \<lbrakk>\<lbrakk>x\<rbrakk>\<cdot>\<lbrakk>y\<rbrakk>\<rbrakk>"
+  and hom_coextensive: "\<lbrakk>x\<rbrakk> \<le> x"
+  and hom_idem [simp]: "\<lbrakk>\<lbrakk>x\<rbrakk>\<rbrakk> = \<lbrakk>x\<rbrakk>"
+  and hom_trancl_inductr: "\<lbrakk>z + y\<cdot>x\<rbrakk> \<le> \<lbrakk>y\<rbrakk> \<Longrightarrow> \<lbrakk>z\<cdot>x\<^sup>+\<rbrakk> \<le> \<lbrakk>y\<rbrakk>"
 
 begin
 
-declare mult_onel [simp]
-  and mult_oner [simp]
-  and par_unitl [simp]
-  and par_unitr [simp]
+  declare mult_onel [simp]
+    and mult_oner [simp]
+    and par_unitl [simp]
+    and par_unitr [simp]
 
-lemma "r \<in> I \<Longrightarrow> r \<parallel> r \<le> r" oops
-lemma "r \<in> I \<Longrightarrow> s \<in> I \<Longrightarrow> r \<le> r \<parallel> s" oops
-lemma "r \<in> I \<Longrightarrow> r\<parallel>(x\<cdot>y) = (r\<parallel>x)\<cdot>(r\<parallel>y)" oops
-lemma "r \<in> I \<Longrightarrow> r\<parallel>x\<^sup>+ \<le> (r\<parallel>x)\<^sup>+" nitpick [timeout = 300] oops
+  definition quintuple :: "'a \<Rightarrow> 'a \<Rightarrow> 'a \<Rightarrow> 'a \<Rightarrow> 'a \<Rightarrow> bool" ("_, _ \<turnstile> \<lbrace>_\<rbrace> _ \<lbrace>_\<rbrace>") where
+    "r, g \<turnstile> \<lbrace>p\<rbrace> c \<lbrace>q\<rbrace> \<equiv> \<lbrakk>p\<cdot>(r\<parallel>c)\<rbrakk> \<le> \<lbrakk>q\<rbrakk> \<and> c \<le> g \<and> r \<in> RG \<and> g \<in> RG"
 
-definition guarantee_relation :: "'a \<Rightarrow> 'a \<Rightarrow> bool" ("_ guar _" [99, 99] 100) where
-  "b guar g \<equiv> g \<in> I \<and> b \<le> g"
+  lemma rg_idem_mult [simp]: "r \<in> RG \<Longrightarrow> r\<cdot>r = r"
+    using rg3[where x = 1 and y = 1 and r = r, simplified] ..
 
-definition jones_quintuples :: "'a \<Rightarrow> 'a \<Rightarrow> 'a \<Rightarrow> 'a \<Rightarrow> 'a \<Rightarrow> bool" ("\<lbrace>_,_\<rbrace>_\<lbrace>_,_\<rbrace>") where
-  "\<lbrace>a, r\<rbrace> b \<lbrace>c, g\<rbrace> \<equiv> \<lbrace>a\<rbrace> r\<parallel>b \<lbrace>c\<rbrace> \<and> r \<in> I \<and> b guar g"
+  lemma rg_idem_par : "r \<in> RG \<Longrightarrow> r \<parallel> r = r"
+    by (metis eq_iff rg1 rg2)
 
-declare mult_onel [simp]
-  and mult_oner [simp]
-  and par_unitl [simp]
-  and par_unitr [simp]
+  lemma [simp]: "x \<le> \<lbrakk>y \<sqinter> z\<rbrakk> \<longleftrightarrow> x \<le> \<lbrakk>y\<rbrakk> \<and> x \<le> \<lbrakk>z\<rbrakk>"
+    by (simp add: hom_meet bin_glb_var)
 
-lemma inv_idem_mult [simp]: "r \<in> I \<Longrightarrow> r\<cdot>r = r"
-  using inv3[where x = 1 and y = 1 and r = r, simplified] ..
+  lemma meet_iso: "x \<le> z \<Longrightarrow> y \<le> w \<Longrightarrow> x \<sqinter> y \<le> z \<sqinter> w"
+    by (metis (full_types) bin_glb_var order_refl order_trans)
 
-lemma inv_idem_par : "r \<in> I \<Longrightarrow> r \<parallel> r = r"
-  by (metis eq_iff inv1 inv2)
+  theorem sequential:
+    assumes "r, g \<turnstile> \<lbrace>p\<rbrace> c1 \<lbrace>q\<rbrace>" and "r, g \<turnstile> \<lbrace>q\<rbrace> c2 \<lbrace>s\<rbrace>"
+    shows "r, g \<turnstile> \<lbrace>p\<rbrace> c1 \<cdot> c2 \<lbrace>s\<rbrace>"
+  proof (simp add: quintuple_def, intro conjI)
+    show "r \<in> RG" and "g \<in> RG"
+      by (metis assms(1) quintuple_def)+
 
-lemma guar_par: "\<lbrakk>b guar g; b' guar g'\<rbrakk> \<Longrightarrow> (b \<parallel> b') guar (g \<parallel> g')"
-  by (metis par_comm par_isol inv_par_closed guarantee_relation_def order_trans)
+    hence "\<lbrakk>p \<cdot> (r \<parallel> c1 \<cdot> c2)\<rbrakk> \<le> \<lbrakk>p \<cdot> ((r \<parallel> c1) \<cdot> (r \<parallel> c2))\<rbrakk>"
+      by (intro hom_iso mult_isol[rule_format]) (metis order_refl rg3)
+    also have "... \<le> \<lbrakk>p \<cdot> (r \<parallel> c1) \<cdot> (r \<parallel> c2)\<rbrakk>"
+      by (metis mult_assoc order_refl)
+    also have "... \<le> \<lbrakk>q \<cdot> (r \<parallel> c2)\<rbrakk>"
+      by (subst hom_mult, subst hom_mult, rule hom_iso, rule mult_isol[rule_format], metis assms(1) quintuple_def)
+    also have "... \<le> \<lbrakk>s\<rbrakk>"
+      by (metis assms(2) quintuple_def)
+    finally show "\<lbrakk>p \<cdot> (r \<parallel> c1 \<cdot> c2)\<rbrakk> \<le> \<lbrakk>s\<rbrakk>" .
 
-theorem paralel_composition:
-  assumes "\<lbrace>a, r\<rbrace> b \<lbrace>c, g\<rbrace>" and "\<lbrace>a', r'\<rbrace> b' \<lbrace>c', g'\<rbrace>"
-  and "g' guar r" and "g guar r'"
-  shows "\<lbrace>a \<sqinter> a', r \<sqinter> r'\<rbrace> b\<parallel>b' \<lbrace>c \<sqinter> c', g\<parallel>g'\<rbrace>"
-proof -
-  have "a\<cdot>(r\<parallel>b) \<le> c" 
-    by (metis assms(1) hoare_triple_def jones_quintuples_def)
-  hence "a\<cdot>((r\<parallel>r)\<parallel>b) \<le> c" 
-    by (metis (full_types) assms(3) par_comm guarantee_relation_def inv_idem_par)
-  hence "a\<cdot>(r\<parallel>(r\<parallel>b)) \<le> c" 
-    by (metis par_comm par_comml)
-  moreover have "b' \<le> r"
-    by (metis assms(2) assms(3) guarantee_relation_def jones_quintuples_def order_trans)
-  ultimately have "a\<cdot>(r\<parallel>(b\<parallel>b')) \<le> c" 
-    by (metis par_assoc par_comm par_isol mult_isor order_trans)
-  hence "(a \<sqinter> a')\<cdot>(r\<parallel>(b\<parallel>b')) \<le> c"
-    by (metis bin_glb_var mult_isol order_refl order_trans)
-  hence one: "(a \<sqinter> a')\<cdot>((r \<sqinter> r')\<parallel>(b\<parallel>b')) \<le> c" 
-    by (metis bin_glb_var par_comm par_isor dual.order_trans eq_refl mult_isor)
+    have "c1 \<cdot> c2 \<le> g \<cdot> g"
+      apply (intro mult_isol_var[rule_format] conjI)
+      apply (metis assms(1) quintuple_def)
+      by (metis assms(2) quintuple_def)
+    also have "... = g"
+      by (metis `g \<in> RG` rg_idem_mult)
+    finally show "c1 \<cdot> c2 \<le> g" .
+  qed
 
-  have "a'\<cdot>(r'\<parallel>b') \<le> c'" 
-    by (metis assms(2) hoare_triple_def jones_quintuples_def)
-  hence "a'\<cdot>((r'\<parallel>r')\<parallel>b') \<le> c'" 
-    by (metis (full_types) assms(2) inv_idem_par jones_quintuples_def)
-  hence "a'\<cdot>(r'\<parallel>(r'\<parallel>b')) \<le> c'"
-    by (metis par_comm par_comml)
-  moreover have "b \<le> r'"
-    by (metis assms(1) assms(4) guarantee_relation_def jones_quintuples_def order_trans)
-  ultimately have "a'\<cdot>(r'\<parallel>(b\<parallel>b')) \<le> c'" 
-    by (metis par_assoc par_comm par_isol mult_isor order_trans)
-  hence "(a \<sqinter> a')\<cdot>(r'\<parallel>(b\<parallel>b')) \<le> c'"
-    by (metis bin_glb_var mult_isol order_refl order_trans)
-  hence two: "(a \<sqinter> a')\<cdot>((r \<sqinter> r')\<parallel>(b\<parallel>b')) \<le> c'"
-    by (metis bin_glb_var par_comm par_isor dual.order_trans eq_refl mult_isor)
-  
-  from one and two have "(a \<sqinter> a')\<cdot>((r \<sqinter> r')\<parallel>(b\<parallel>b')) \<le> c \<sqinter> c'"
-    by (metis bin_glb_var)
-  moreover have "(b\<parallel>b') guar (g\<parallel>g')"
-    by (metis assms(1) assms(2) guar_par jones_quintuples_def)
-  ultimately show ?thesis
-    by (metis (full_types) assms(1) assms(2) hoare_triple_def jones_quintuples_def inv_meet_closed)
-qed
+  theorem parallel:
+    assumes "r1, g1 \<turnstile> \<lbrace>p1\<rbrace> c1 \<lbrace>q1\<rbrace>" and "g2 \<le> r1"
+    and "r2, g2 \<turnstile> \<lbrace>p2\<rbrace> c2 \<lbrace>q2\<rbrace>" and "g1 \<le> r2"
+    shows "(r1 \<sqinter> r2), (g1 \<parallel> g2) \<turnstile> \<lbrace>p1 \<sqinter> p2\<rbrace> c1 \<parallel> c2 \<lbrace>q1 \<sqinter> q2\<rbrace>"
+  proof (simp add: quintuple_def, intro conjI)
+    have "r1 \<in> RG" and "r2 \<in> RG" and "g1 \<in> RG" and "g2 \<in> RG"
+      by (metis assms(1) assms(3) quintuple_def)+
 
-theorem sequential_composition:
-  assumes "\<lbrace>a, r\<rbrace> b \<lbrace>c, g\<rbrace>" and "\<lbrace>c, r'\<rbrace> b' \<lbrace>c', g'\<rbrace>"
-  shows "\<lbrace>a, r \<sqinter> r'\<rbrace> b\<cdot>b' \<lbrace>c', g\<parallel>g'\<rbrace>"
-proof -
-  have "b\<cdot>b' \<le> g\<cdot>g'"
-    by (metis assms(1) assms(2) guarantee_relation_def jones_quintuples_def mult_isol_var)
-  hence guarantee: "(b\<cdot>b') guar (g\<parallel>g')"
-    by (metis (full_types) assms(1) assms(2) guarantee_relation_def inv_mult_par inv_par_closed jones_quintuples_def order_trans)
-  have "(r \<sqinter> r') \<in> I"
-    by (metis assms(1) assms(2) jones_quintuples_def inv_meet_closed)
-  hence "(r \<sqinter> r')\<parallel>(b\<cdot>b') \<le> ((r \<sqinter> r')\<parallel>b)\<cdot>((r \<sqinter> r')\<parallel>b')"
-    by (insert inv_def[of "r \<sqinter> r'" b "b'"], simp)
-  also have "... \<le> (r\<parallel>b)\<cdot>(r'\<parallel>b')"
-    by (metis bin_glb_var par_comm par_isor dual.order_trans eq_refl mult_isol mult_isor)
-  finally have "(r \<sqinter> r')\<parallel>(b\<cdot>b') \<le> (r\<parallel>b)\<cdot>(r'\<parallel>b')"
-    by (metis)
-  hence "\<lbrace>a\<rbrace>(r \<sqinter> r')\<parallel>(b\<cdot>b')\<lbrace>c'\<rbrace>"
-    by (metis assms(1) assms(2) comp_antitony jones_quintuples_def)
-  thus ?thesis using guarantee
-    by (metis assms(1) assms(2) jones_quintuples_def inv_meet_closed)
-qed
+    have "\<lbrakk>(p1 \<sqinter> p2) \<cdot> ((r1 \<sqinter> r2) \<parallel> (c1 \<parallel> c2))\<rbrakk> \<le> \<lbrakk>p1 \<cdot> ((r1 \<sqinter> r2) \<parallel> (c1 \<parallel> c2))\<rbrakk>"
+      by (metis bin_glb_var hom_iso mult_isol order_refl par_comm)
+    also have "... \<le> \<lbrakk>p1 \<cdot> ((r1 \<sqinter> r2) \<parallel> (c1 \<parallel> g2))\<rbrakk>"
+      by (intro hom_iso mult_isol_var[rule_format] par_double_iso[rule_format] conjI order_refl) (metis assms(3) quintuple_def)
+    also have "... \<le> \<lbrakk>p1 \<cdot> (r1 \<parallel> (c1 \<parallel> r1))\<rbrakk>"
+      by (intro hom_iso mult_isol_var[rule_format] conjI order_refl) (metis assms(2) bin_glb_var eq_refl par_double_iso)
+    also have "... \<le> \<lbrakk>p1 \<cdot> (r1 \<parallel> c1)\<rbrakk>"
+      by (intro hom_iso mult_isor[rule_format])  (metis `r1 \<in> RG` eq_iff par_assoc par_comm rg_idem_par)
+    also have "... \<le> \<lbrakk>q1\<rbrakk>"
+      by (metis assms(1) quintuple_def)
+    finally show "\<lbrakk>(p1 \<sqinter> p2) \<cdot> (r1 \<sqinter> r2 \<parallel> (c1 \<parallel> c2))\<rbrakk> \<le> \<lbrakk>q1\<rbrakk>" .
 
-theorem rg_one: "\<lbrace>a, r\<rbrace> 1 \<lbrace>c, g\<rbrace> \<longleftrightarrow> \<lbrace>a\<rbrace> r \<lbrace>c\<rbrace> \<and> r \<in> I \<and> g \<in> I"
-  by (metis par_unitr guarantee_relation_def inv_def jones_quintuples_def)
+    have "\<lbrakk>(p1 \<sqinter> p2) \<cdot> (r1 \<sqinter> r2 \<parallel> (c1 \<parallel> c2))\<rbrakk> \<le> \<lbrakk>p2 \<cdot> (r1 \<sqinter> r2 \<parallel> (c1 \<parallel> c2))\<rbrakk>"
+      by (metis bin_glb_var hom_iso mult_isol order_refl)
+    also have "... \<le> \<lbrakk>p2 \<cdot> (r1 \<sqinter> r2 \<parallel> (g1 \<parallel> c2))\<rbrakk>"
+      by (intro mult_isol_var[rule_format] conjI order_refl hom_iso par_double_iso[rule_format]) (metis assms(1) quintuple_def)
+    also have "... \<le> \<lbrakk>p2 \<cdot> (r2 \<parallel> (r2 \<parallel> c2))\<rbrakk>"
+      by (intro mult_isol_var[rule_format] hom_iso conjI order_refl) (metis assms(4) bin_glb_var order_refl par_double_iso)
+    also have "... \<le> \<lbrakk>p2 \<cdot> (r2 \<parallel> c2)\<rbrakk>"
+      by (intro hom_iso mult_isor[rule_format]) (metis `r2 \<in> RG` eq_iff par_comm par_comml rg_idem_par)
+    also have "... \<le> \<lbrakk>q2\<rbrakk>"
+      by (metis assms(3) quintuple_def)
+    finally show "\<lbrakk>(p1 \<sqinter> p2) \<cdot> (r1 \<sqinter> r2 \<parallel> (c1 \<parallel> c2))\<rbrakk> \<le> \<lbrakk>q2\<rbrakk>" .
 
-theorem rg_add: "\<lbrace>a, r\<rbrace> b + b' \<lbrace>c, g\<rbrace> \<longleftrightarrow> \<lbrace>a, r\<rbrace> b \<lbrace>c, g\<rbrace> \<and> \<lbrace>a, r\<rbrace> b' \<lbrace>c, g\<rbrace>"
-proof (default, metis (full_types) add_lub par_distl choice guarantee_relation_def jones_quintuples_def)
-  assume assms: "\<lbrace>a, r\<rbrace> b \<lbrace>c, g\<rbrace> \<and> \<lbrace>a, r\<rbrace> b' \<lbrace>c, g\<rbrace>"
-  hence "r \<in> I \<and> (b + b') guar g"
-    by (metis (full_types) add_lub guarantee_relation_def jones_quintuples_def)
-  moreover have "\<lbrace>a\<rbrace> r \<parallel> (b + b') \<lbrace>c\<rbrace>"
-    by (metis assms par_distl choice jones_quintuples_def)
-  ultimately show "\<lbrace>a, r\<rbrace> b + b' \<lbrace>c, g\<rbrace>"
-    by (metis jones_quintuples_def)
-qed
+    show "c1 \<parallel> c2 \<le> g1 \<parallel> g2"
+      by (rule par_double_iso[rule_format]) (metis assms(1) quintuple_def assms(3))
 
-lemma one_trancl: "1\<^sup>+ = 1"
-  by (metis mult_oner star_one star_trancl)
+    show "r1 \<sqinter> r2 \<in> RG"
+      by (metis `r1 \<in> RG` `r2 \<in> RG` rg_meet_closed)
+    show "g1 \<parallel> g2 \<in> RG"
+      by (metis `g1 \<in> RG` `g2 \<in> RG` rg_par_closed)
+  qed
 
-lemma inv_plus_eq: "r \<in> I \<Longrightarrow> r = r\<^sup>+"
-  by (metis inv_idem_mult star_inductr_var_eq2 star_trancl)
-
-lemma inv_def_var: "r \<in> I \<Longrightarrow> (r\<parallel>x)\<^sup>+ = r\<parallel>x\<^sup>+"
-  by (metis inv_def)
-
-lemma guar_trancl: "b guar g \<Longrightarrow> b\<^sup>+ guar g"
-  apply (simp only: guarantee_relation_def)
-  apply (subgoal_tac "1 + g \<cdot> b \<le> g")
-  apply (metis mult_onel trancl_inductr)
-  by (metis add_commute add_iso inv_def inv_idem_mult leq_def mult_isor)
-
-theorem rg_transcl: "\<lbrace>a, r\<rbrace> b \<lbrace>a, g\<rbrace> \<Longrightarrow> \<lbrace>a, r\<rbrace> b\<^sup>+ \<lbrace>a, g\<rbrace>"
-  by (metis guar_trancl inv_def iteration2 jones_quintuples_def)
-
-theorem rg_star: "\<lbrakk>\<lbrace>a\<rbrace> r \<lbrace>a\<rbrace>; \<lbrace>a, r\<rbrace> b \<lbrace>a, g\<rbrace>\<rbrakk> \<Longrightarrow> \<lbrace>a, r\<rbrace> b\<^sup>* \<lbrace>a, g\<rbrace>"
-  by (metis star_trancl2 guarantee_relation_def jones_quintuples_def rg_add rg_one rg_transcl)
+  theorem rg_star: "\<lbrakk>\<lbrakk>p\<cdot>r\<rbrakk> \<le> \<lbrakk>p\<rbrakk>; r, g \<turnstile> \<lbrace>p\<rbrace> c \<lbrace>p\<rbrace>\<rbrakk> \<Longrightarrow> r, g \<turnstile> \<lbrace>p\<rbrace> c\<^sup>* \<lbrace>p\<rbrace>"
+    apply (simp add: quintuple_def)
+    apply (intro conjI)
+    apply (erule conjE)+
+    apply (simp add: star_trancl2 par_distl mult_distl add_lub)
+    apply (rule order_trans[where y = "\<lbrakk>p \<cdot> (r \<parallel> c)\<^sup>+\<rbrakk>"])
+    apply (metis hom_iso mult_isor rg4)
+    apply (rule hom_trancl_inductr)
+    apply (simp add: add_lub)
+    by (metis leq_def par_unitl rg2 rg_idem_mult rg_unit star_iso star_rtc3)
 
 end
 
